Implement SAR #40
This puts through two implementations of the SAR bytecode.  One follows
the yellow paper, whilst the other uses bitshifts.  The latter appears
to perform significantly better when translated into Java.

src/test/java/dafnyevm/Tests.java
@@ -14,6 +14,7 @@
 package dafnyevm;
 import java.math.BigInteger;
 import java.util.HashMap;
+import java.util.Arrays;
 
 import org.junit.jupiter.api.Test;
 
@@ -744,7 +745,61 @@ public class Tests {
 		assertArrayEquals(UINT256(0x7F0), output);
 	}
 
-	// Add more shift tests here!
+	@Test
+	public void test_shr_01() {
+		// 0x1FC >> 1 = 0xFE
+		byte[] output = call(new int[] { PUSH2, 0x1, 0xFC, PUSH1, 0x1, SHR, PUSH1, 0x00, MSTORE, PUSH1, 0x20, PUSH1, 0x00, RETURN });
+		assertArrayEquals(UINT256(0xFE), output);
+	}
+
+	@Test
+	public void test_shr_02() {
+		// 0x3F8 >> 2 = 0xFE
+		byte[] output = call(new int[] { PUSH2, 0x3, 0xF8, PUSH1, 0x2, SHR, PUSH1, 0x00, MSTORE, PUSH1, 0x20, PUSH1, 0x00, RETURN });
+		assertArrayEquals(UINT256(0xFE), output);
+	}
+
+	@Test
+	public void test_shr_03() {
+		// 0x7F0 >> 3 = 0xFE
+		byte[] output = call(new int[] { PUSH2, 0x7, 0xF0, PUSH1, 0x3, SHR, PUSH1, 0x00, MSTORE, PUSH1, 0x20, PUSH1, 0x00, RETURN });
+		assertArrayEquals(UINT256(0xFE), output);
+	}
+
+	@Test
+	public void test_sar_01() {
+		// (0 - 0x2) >> 1 = -0x1
+		byte[] output = call(new int[] { PUSH1, 0x2, PUSH1, 0x0, SUB, PUSH1, 0x1, SAR, PUSH1, 0x00, MSTORE, PUSH1, 0x20, PUSH1, 0x00, RETURN });
+		assertArrayEquals(INT256(-0x1), output);
+	}
+
+	@Test
+	public void test_sar_02() {
+		// 0x1FC >> 1 = 0xFE
+		byte[] output = call(new int[] { PUSH2, 0x1, 0xFC, PUSH1, 0x1, SAR, PUSH1, 0x00, MSTORE, PUSH1, 0x20, PUSH1, 0x00, RETURN });
+		assertArrayEquals(UINT256(0xFE), output);
+	}
+
+	@Test
+	public void test_sar_03() {
+		// (0 - 0x1FC) >> 1 = -0xFE
+		byte[] output = call(new int[] { PUSH2, 0x1, 0xFC, PUSH1, 0x0, SUB, PUSH1, 0x1, SAR, PUSH1, 0x00, MSTORE, PUSH1, 0x20, PUSH1, 0x00, RETURN });
+		assertArrayEquals(INT256(-0xFE), output);
+	}
+
+	@Test
+	public void test_sar_04() {
+		// (0 - 0x3F8) >> 2 = -0xFE
+		byte[] output = call(new int[] { PUSH2, 0x3, 0xF8, PUSH1, 0x0, SUB, PUSH1, 0x2, SAR, PUSH1, 0x00, MSTORE, PUSH1, 0x20, PUSH1, 0x00, RETURN });
+		assertArrayEquals(INT256(-0xFE), output);
+	}
+
+	@Test
+	public void test_sar_05() {
+		// (0 - 0x7F0) >> 3 = -0xFE
+		byte[] output = call(new int[] { PUSH2, 0x7, 0xF0, PUSH1, 0x0, SUB, PUSH1, 0x3, SAR, PUSH1, 0x00, MSTORE, PUSH1, 0x20, PUSH1, 0x00, RETURN });
+		assertArrayEquals(INT256(-0xFE), output);
+	}
 
 	// ========================================================================
 	// LT / GT / SLT / SGT / EQ / ISZERO
@@ -1575,6 +1630,25 @@ public class Tests {
 		bytes[29] = (byte) ((x >> 16) & 0xFF);
 		bytes[28] = (byte) ((x >> 24) & 0xFF);
 		return bytes;
+	}
+
+	/**
+	 * Construct a 256bit representation (in big endian form) of a signed Java int.
+	 * @param x
+	 * @return
+	 */
+	private byte[] INT256(int x) {
+		if (x >= 0) {
+			return UINT256(x);
+		} else {
+			byte[] bytes = new byte[32];
+			Arrays.fill(bytes, 0, 31, (byte) 0xff);
+			bytes[31] = (byte) (x & 0xFF);
+			bytes[30] = (byte) ((x >> 8) & 0xFF);
+			bytes[29] = (byte) ((x >> 16) & 0xFF);
+			bytes[28] = (byte) ((x >> 24) & 0xFF);
+			return bytes;
+		}
 	}
 
 	/**
