src/dafny/util/int.dfy
@@ -12,123 +12,123 @@
  * under the License.
  */
 module Int {
-  // Powers of Two
-  const TWO_7   : int := 0x0_80;
-  const TWO_8   : int := 0x1_00;
-  const TWO_15  : int := 0x0_8000;
-  const TWO_16  : int := 0x1_0000;
-  const TWO_24  : int := 0x1_0000_00;
-  const TWO_31  : int := 0x0_8000_0000;
-  const TWO_32  : int := 0x1_0000_0000;
-  const TWO_40  : int := 0x1_0000_0000_00;
-  const TWO_48  : int := 0x1_0000_0000_0000;
-  const TWO_56  : int := 0x1_0000_0000_0000_00;
-  const TWO_63  : int := 0x0_8000_0000_0000_0000;
-  const TWO_64  : int := 0x1_0000_0000_0000_0000;
-  const TWO_127 : int := 0x0_8000_0000_0000_0000_0000_0000_0000_0000;
-  const TWO_128 : int := 0x1_0000_0000_0000_0000_0000_0000_0000_0000;
-  const TWO_160 : int := 0x1_0000_0000_0000_0000_0000_0000_0000_0000_0000_0000;
-  const TWO_255 : int := 0x0_8000_0000_0000_0000_0000_0000_0000_0000_0000_0000_0000_0000_0000_0000_0000_0000;
-  const TWO_256 : int := 0x1_0000_0000_0000_0000_0000_0000_0000_0000_0000_0000_0000_0000_0000_0000_0000_0000;
+    // Powers of Two
+    const TWO_7   : int := 0x0_80;
+    const TWO_8   : int := 0x1_00;
+    const TWO_15  : int := 0x0_8000;
+    const TWO_16  : int := 0x1_0000;
+    const TWO_24  : int := 0x1_0000_00;
+    const TWO_31  : int := 0x0_8000_0000;
+    const TWO_32  : int := 0x1_0000_0000;
+    const TWO_40  : int := 0x1_0000_0000_00;
+    const TWO_48  : int := 0x1_0000_0000_0000;
+    const TWO_56  : int := 0x1_0000_0000_0000_00;
+    const TWO_63  : int := 0x0_8000_0000_0000_0000;
+    const TWO_64  : int := 0x1_0000_0000_0000_0000;
+    const TWO_127 : int := 0x0_8000_0000_0000_0000_0000_0000_0000_0000;
+    const TWO_128 : int := 0x1_0000_0000_0000_0000_0000_0000_0000_0000;
+    const TWO_160 : int := 0x1_0000_0000_0000_0000_0000_0000_0000_0000_0000_0000;
+    const TWO_255 : int := 0x0_8000_0000_0000_0000_0000_0000_0000_0000_0000_0000_0000_0000_0000_0000_0000_0000;
+    const TWO_256 : int := 0x1_0000_0000_0000_0000_0000_0000_0000_0000_0000_0000_0000_0000_0000_0000_0000_0000;
 
-  // Signed Integers
-  const MIN_I8   : int := -TWO_7;
-  const MAX_I8   : int :=  TWO_7 - 1;
-  const MIN_I16  : int := -TWO_15;
-  const MAX_I16  : int :=  TWO_15 - 1;
-  const MIN_I32  : int := -TWO_31;
-  const MAX_I32  : int :=  TWO_31 - 1;
-  const MIN_I64  : int := -TWO_63;
-  const MAX_I64  : int :=  TWO_63 - 1;
-  const MIN_I128 : int := -TWO_127;
-  const MAX_I128 : int :=  TWO_127 - 1;
-  const MIN_I256 : int := -TWO_255;
-  const MAX_I256 : int :=  TWO_255 - 1;
+    // Signed Integers
+    const MIN_I8   : int := -TWO_7;
+    const MAX_I8   : int :=  TWO_7 - 1;
+    const MIN_I16  : int := -TWO_15;
+    const MAX_I16  : int :=  TWO_15 - 1;
+    const MIN_I32  : int := -TWO_31;
+    const MAX_I32  : int :=  TWO_31 - 1;
+    const MIN_I64  : int := -TWO_63;
+    const MAX_I64  : int :=  TWO_63 - 1;
+    const MIN_I128 : int := -TWO_127;
+    const MAX_I128 : int :=  TWO_127 - 1;
+    const MIN_I256 : int := -TWO_255;
+    const MAX_I256 : int :=  TWO_255 - 1;
 
-  newtype{:nativeType "sbyte"} i8 = i:int   | MIN_I8 <= i <= MAX_I8
-  newtype{:nativeType "short"} i16 = i:int  | MIN_I16 <= i <= MAX_I16
-  newtype{:nativeType "int"}   i32 = i:int  | MIN_I32 <= i <= MAX_I32
-  newtype{:nativeType "long"}  i64 = i:int  | MIN_I64 <= i <= MAX_I64
-  newtype i128 = i:int | MIN_I128 <= i <= MAX_I128
-  newtype i256 = i:int | MIN_I256 <= i <= MAX_I256
+    newtype{:nativeType "sbyte"} i8 = i:int   | MIN_I8 <= i <= MAX_I8
+    newtype{:nativeType "short"} i16 = i:int  | MIN_I16 <= i <= MAX_I16
+    newtype{:nativeType "int"}   i32 = i:int  | MIN_I32 <= i <= MAX_I32
+    newtype{:nativeType "long"}  i64 = i:int  | MIN_I64 <= i <= MAX_I64
+    newtype i128 = i:int | MIN_I128 <= i <= MAX_I128
+    newtype i256 = i:int | MIN_I256 <= i <= MAX_I256
 
-  // Unsigned Integers
-  const MAX_U8 : int :=  TWO_8 - 1;
-  const MAX_U16 : int := TWO_16 - 1;
-  const MAX_U24 : int := TWO_24 - 1;
-  const MAX_U32 : int := TWO_32 - 1;
-  const MAX_U40 : int := TWO_40 - 1;
-  const MAX_U48 : int := TWO_48 - 1;
-  const MAX_U56 : int := TWO_56 - 1;
-  const MAX_U64 : int := TWO_64 - 1;
-  const MAX_U128 : int := TWO_128 - 1;
-  const MAX_U160: int := TWO_160 - 1;
-  const MAX_U256: int := TWO_256 - 1
+    // Unsigned Integers
+    const MAX_U8 : int :=  TWO_8 - 1;
+    const MAX_U16 : int := TWO_16 - 1;
+    const MAX_U24 : int := TWO_24 - 1;
+    const MAX_U32 : int := TWO_32 - 1;
+    const MAX_U40 : int := TWO_40 - 1;
+    const MAX_U48 : int := TWO_48 - 1;
+    const MAX_U56 : int := TWO_56 - 1;
+    const MAX_U64 : int := TWO_64 - 1;
+    const MAX_U128 : int := TWO_128 - 1;
+    const MAX_U160: int := TWO_160 - 1;
+    const MAX_U256: int := TWO_256 - 1
 
-  newtype{:nativeType "byte"} u8 = i:int    | 0 <= i <= MAX_U8
-  newtype{:nativeType "ushort"} u16 = i:int | 0 <= i <= MAX_U16
-  newtype{:nativeType "uint"} u24 = i:int | 0 <= i <= MAX_U24
-  newtype{:nativeType "uint"} u32 = i:int   | 0 <= i <= MAX_U32
-  newtype{:nativeType "ulong"} u40 = i:int   | 0 <= i <= MAX_U40
-  newtype{:nativeType "ulong"} u48 = i:int   | 0 <= i <= MAX_U48
-  newtype{:nativeType "ulong"} u56 = i:int   | 0 <= i <= MAX_U56
-  newtype{:nativeType "ulong"} u64 = i:int  | 0 <= i <= MAX_U64
-  newtype u128 = i:int | 0 <= i <= MAX_U128
-  newtype u160 = i:int | 0 <= i <= MAX_U160
-  newtype u256 = i:int | 0 <= i <= MAX_U256
+    newtype{:nativeType "byte"} u8 = i:int    | 0 <= i <= MAX_U8
+    newtype{:nativeType "ushort"} u16 = i:int | 0 <= i <= MAX_U16
+    newtype{:nativeType "uint"} u24 = i:int | 0 <= i <= MAX_U24
+    newtype{:nativeType "uint"} u32 = i:int   | 0 <= i <= MAX_U32
+    newtype{:nativeType "ulong"} u40 = i:int   | 0 <= i <= MAX_U40
+    newtype{:nativeType "ulong"} u48 = i:int   | 0 <= i <= MAX_U48
+    newtype{:nativeType "ulong"} u56 = i:int   | 0 <= i <= MAX_U56
+    newtype{:nativeType "ulong"} u64 = i:int  | 0 <= i <= MAX_U64
+    newtype u128 = i:int | 0 <= i <= MAX_U128
+    newtype u160 = i:int | 0 <= i <= MAX_U160
+    newtype u256 = i:int | 0 <= i <= MAX_U256
 
 
-  // Determine maximum of two u256 integers.
-  function method Max(i1: int, i2: int) : int {
-    if i1 >= i2 then i1 else i2
-  }
+    // Determine maximum of two u256 integers.
+    function method Max(i1: int, i2: int) : int {
+        if i1 >= i2 then i1 else i2
+    }
 
-  // Round up a given number (i) by a given multiple (r).
-  function method RoundUp(i: int, r: nat) : int
-  requires r > 0 {
-    if (i % r) == 0 then i
-    else
-      ((i/r)*r) + r
-  }
+    // Round up a given number (i) by a given multiple (r).
+    function method RoundUp(i: int, r: nat) : int
+    requires r > 0 {
+        if (i % r) == 0 then i
+        else
+        ((i/r)*r) + r
+    }
 
-  // =========================================================
-  // Conversion to/from byte sequences
-  // =========================================================
+    // =========================================================
+    // Conversion to/from byte sequences
+    // =========================================================
 
-  function method ReadUint8(bytes: seq<u8>, address:nat) : u8
-  requires address < |bytes| {
-    bytes[address]
-  }
+    function method ReadUint8(bytes: seq<u8>, address:nat) : u8
+    requires address < |bytes| {
+        bytes[address]
+    }
 
-  function method ReadUint16(bytes: seq<u8>, address:nat) : u16
-  requires (address+1) < |bytes| {
-    var b1 := bytes[address] as u16;
-    var b2 := bytes[address+1] as u16;
-    (b1 * (TWO_8 as u16)) + b2
-  }
+    function method ReadUint16(bytes: seq<u8>, address:nat) : u16
+    requires (address+1) < |bytes| {
+        var b1 := bytes[address] as u16;
+        var b2 := bytes[address+1] as u16;
+        (b1 * (TWO_8 as u16)) + b2
+    }
 
-  function method ReadUint32(bytes: seq<u8>, address:nat) : u32
-  requires (address+3) < |bytes| {
-    var b1 := ReadUint16(bytes, address) as u32;
-    var b2 := ReadUint16(bytes, address+2) as u32;
-    (b1 * (TWO_16 as u32)) + b2
-  }
+    function method ReadUint32(bytes: seq<u8>, address:nat) : u32
+    requires (address+3) < |bytes| {
+        var b1 := ReadUint16(bytes, address) as u32;
+        var b2 := ReadUint16(bytes, address+2) as u32;
+        (b1 * (TWO_16 as u32)) + b2
+    }
 
-  function method ReadUint64(bytes: seq<u8>, address:nat) : u64
-  requires (address+7) < |bytes| {
-    var b1 := ReadUint32(bytes, address) as u64;
-    var b2 := ReadUint32(bytes, address+4) as u64;
-    (b1 * (TWO_32 as u64)) + b2
-  }
+    function method ReadUint64(bytes: seq<u8>, address:nat) : u64
+    requires (address+7) < |bytes| {
+        var b1 := ReadUint32(bytes, address) as u64;
+        var b2 := ReadUint32(bytes, address+4) as u64;
+        (b1 * (TWO_32 as u64)) + b2
+    }
 
-  // =========================================================
-  // Exponent
-  // =========================================================
+    // =========================================================
+    // Exponent
+    // =========================================================
 
     /**
      * Compute n^k.
      */
-    function method Pow(n:nat, k:nat) : int {
+    function method Pow(n:nat, k:nat) : nat {
         if k == 0 then 1
         else if k == 1 then n
         else
@@ -138,300 +138,353 @@ module Int {
             else np * np * n
     }
 
-  // Various sanity tests for exponentiation.
-  method PowTests() {
-    assert Pow(2,8) == TWO_8;
-    assert Pow(2,15) == TWO_15;
-    assert Pow(2,16) == TWO_16;
-    assert Pow(2,24) == TWO_24;
-    assert Pow(2,31) == TWO_31;
-    assert Pow(2,32) == TWO_32;
-    assert Pow(2,40) == TWO_40;
-    assert Pow(2,48) == TWO_48;
-    assert Pow(2,56) == TWO_56;
-    assert Pow(2,63) == TWO_63;
-    assert Pow(2,64) == TWO_64;
-    // NOTE:  I have to break the following ones up because Z3
-    // cannot handle it.
-    assert Pow(2,63) * Pow(2,64) == TWO_127;
-    assert Pow(2,64) * Pow(2,64) == TWO_128;
-    assert Pow(2,64) * Pow(2,64) * Pow(2,64) * Pow(2,64) == TWO_256;
-    assert (TWO_128 / TWO_64) == TWO_64;
-    assert (TWO_256 / TWO_128) == TWO_128;
-  }
+    // Simple lemma about POW.
+    lemma lemma_pow2(k:nat)
+    ensures Pow(2,k) > 0 {
+        if k == 0 {
+            assert Pow(2,k) == 1;
+        } else if k == 1 {
+            assert Pow(2,k) == 2;
+        } else {
+            lemma_pow2(k/2);
+        }
+    }
 
-  // =========================================================
-  // Non-Euclidean Division / Remainder
-  // =========================================================
+    // Various sanity tests for exponentiation.
+    method PowTests() {
+        assert Pow(2,8) == TWO_8;
+        assert Pow(2,15) == TWO_15;
+        assert Pow(2,16) == TWO_16;
+        assert Pow(2,24) == TWO_24;
+        assert Pow(2,31) == TWO_31;
+        assert Pow(2,32) == TWO_32;
+        assert Pow(2,40) == TWO_40;
+        assert Pow(2,48) == TWO_48;
+        assert Pow(2,56) == TWO_56;
+        assert Pow(2,63) == TWO_63;
+        assert Pow(2,64) == TWO_64;
+        // NOTE:  I have to break the following ones up because Z3
+        // cannot handle it.
+        assert Pow(2,63) * Pow(2,64) == TWO_127;
+        assert Pow(2,64) * Pow(2,64) == TWO_128;
+        assert Pow(2,64) * Pow(2,64) * Pow(2,64) * Pow(2,64) == TWO_256;
+        assert (TWO_128 / TWO_64) == TWO_64;
+        assert (TWO_256 / TWO_128) == TWO_128;
+    }
 
-  // This provides a non-Euclidean division operator and is necessary
-  // because Dafny (unlike just about every other programming
-  // language) supports Euclidean division.  This operator, therefore,
-  // always divides *towards* zero.
-  function method Div(lhs: int, rhs: int) : int
-  requires rhs != 0 {
-    if lhs >= 0 then lhs / rhs
-    else
-      -((-lhs) / rhs)
-  }
+    // =========================================================
+    // Non-Euclidean Division / Remainder
+    // =========================================================
 
-  // This provides a non-Euclidean Remainder operator and is necessary
-  // because Dafny (unlike just about every other programming
-  // language) supports Euclidean division.  Observe that this is a
-  // true Remainder operator, and not a modulus operator.  For
-  // emxaple, this means the result can be negative.
-  function method Rem(lhs: int, rhs: int) : int
-  requires rhs != 0 {
-    if lhs >= 0 then (lhs % rhs)
-    else
-      var d := -((-lhs) / rhs);
-      lhs - (d * rhs)
-  }
+    // This provides a non-Euclidean division operator and is necessary
+    // because Dafny (unlike just about every other programming
+    // language) supports Euclidean division.  This operator, therefore,
+    // always divides *towards* zero.
+    function method Div(lhs: int, rhs: int) : int
+    requires rhs != 0 {
+        if lhs >= 0 then lhs / rhs
+        else
+        -((-lhs) / rhs)
+    }
 
-  // Various sanity tests for division.
-  method DivTests() {
-    // pos-pos
-    assert Div(6,2) == 3;
-    assert Div(6,3) == 2;
-    assert Div(6,4) == 1;
-    assert Div(9,4) == 2;
-    // neg-pos
-    assert Div(-6,2) == -3;
-    assert Div(-6,3) == -2;
-    assert Div(-6,4) == -1;
-    assert Div(-9,4) == -2;
-    // pos-neg
-    assert Div(6,-2) == -3;
-    assert Div(6,-3) == -2;
-    assert Div(6,-4) == -1;
-    assert Div(9,-4) == -2;
-    // neg-neg
-    assert Div(-6,-2) == 3;
-    assert Div(-6,-3) == 2;
-    assert Div(-6,-4) == 1;
-    assert Div(-9,-4) == 2;
-  }
+    // This provides a non-Euclidean Remainder operator and is necessary
+    // because Dafny (unlike just about every other programming
+    // language) supports Euclidean division.  Observe that this is a
+    // true Remainder operator, and not a modulus operator.  For
+    // emxaple, this means the result can be negative.
+    function method Rem(lhs: int, rhs: int) : int
+    requires rhs != 0 {
+        if lhs >= 0 then (lhs % rhs)
+        else
+        var d := -((-lhs) / rhs);
+        lhs - (d * rhs)
+    }
 
-  // Various sanity tests for Remainder.
-  method RemTests() {
-    // pos-pos
-    assert Rem(6,2) == 0;
-    assert Rem(6,3) == 0;
-    assert Rem(6,4) == 2;
-    assert Rem(9,4) == 1;
-    // neg-pos
-    assert Rem(-6,2) == 0;
-    assert Rem(-6,3) == 0;
-    assert Rem(-6,4) == -2;
-    assert Rem(-9,4) == -1;
-    // pos-neg
-    assert Rem(6,-2) == 0;
-    assert Rem(6,-3) == 0;
-    assert Rem(6,-4) == 2;
-    assert Rem(9,-4) == 1;
-    // neg-neg
-    assert Rem(-6,-2) == 0;
-    assert Rem(-6,-3) == 0;
-    assert Rem(-6,-4) == -2;
-    assert Rem(-9,-4) == -1;
-  }
-}
+    // Various sanity tests for division.
+    method DivTests() {
+        // pos-pos
+        assert Div(6,2) == 3;
+        assert Div(6,3) == 2;
+        assert Div(6,4) == 1;
+        assert Div(9,4) == 2;
+        // neg-pos
+        assert Div(-6,2) == -3;
+        assert Div(-6,3) == -2;
+        assert Div(-6,4) == -1;
+        assert Div(-9,4) == -2;
+        // pos-neg
+        assert Div(6,-2) == -3;
+        assert Div(6,-3) == -2;
+        assert Div(6,-4) == -1;
+        assert Div(9,-4) == -2;
+        // neg-neg
+        assert Div(-6,-2) == 3;
+        assert Div(-6,-3) == 2;
+        assert Div(-6,-4) == 1;
+        assert Div(-9,-4) == 2;
+    }
+
+    // Various sanity tests for Remainder.
+    method RemTests() {
+        // pos-pos
+        assert Rem(6,2) == 0;
+        assert Rem(6,3) == 0;
+        assert Rem(6,4) == 2;
+        assert Rem(9,4) == 1;
+        // neg-pos
+        assert Rem(-6,2) == 0;
+        assert Rem(-6,3) == 0;
+        assert Rem(-6,4) == -2;
+        assert Rem(-9,4) == -1;
+        // pos-neg
+        assert Rem(6,-2) == 0;
+        assert Rem(6,-3) == 0;
+        assert Rem(6,-4) == 2;
+        assert Rem(9,-4) == 1;
+        // neg-neg
+        assert Rem(-6,-2) == 0;
+        assert Rem(-6,-3) == 0;
+        assert Rem(-6,-4) == -2;
+        assert Rem(-9,-4) == -1;
+    }
+    }
 
 /**
  * Various helper methods related to unsigned 16bit integers.
  */
 module U16 {
-  import opened Int
+    import opened Int
 
-  // Read nth 8bit word (i.e. byte) out of this u16, where 0
-  // identifies the most significant byte.
-  function method NthUint8(v:u16, k: nat) : u8
-    // Cannot read more than two words!
-  requires k < 2 {
-    if k == 0
-        then (v / (TWO_8 as u16)) as u8
-      else
-        (v % (TWO_8 as u16)) as u8
-  }
+    // Read nth 8bit word (i.e. byte) out of this u16, where 0
+    // identifies the most significant byte.
+    function method NthUint8(v:u16, k: nat) : u8
+        // Cannot read more than two words!
+    requires k < 2 {
+        if k == 0
+            then (v / (TWO_8 as u16)) as u8
+        else
+            (v % (TWO_8 as u16)) as u8
+    }
 
-  method tests_NthUint8() {
-    assert NthUint8(0xde80,0) == 0xde;
-    assert NthUint8(0xde80,1) == 0x80;
-  }
+    method tests_NthUint8() {
+        assert NthUint8(0xde80,0) == 0xde;
+        assert NthUint8(0xde80,1) == 0x80;
+    }
 }
 
 /**
  * Various helper methods related to unsigned 32bit integers.
  */
 module U32 {
-  import opened Int
+    import opened Int
 
-  // Read nth 16bit word out of this u32, where 0 identifies the most
-  // significant word.
-  function method NthUint16(v:u32, k: nat) : u16
-    // Cannot read more than two words!
-  requires k < 2 {
-    if k == 0
-        then (v / (TWO_16 as u32)) as u16
-      else
-        (v % (TWO_16 as u32)) as u16
-  }
+    // Read nth 16bit word out of this u32, where 0 identifies the most
+    // significant word.
+    function method NthUint16(v:u32, k: nat) : u16
+        // Cannot read more than two words!
+    requires k < 2 {
+        if k == 0
+            then (v / (TWO_16 as u32)) as u16
+        else
+            (v % (TWO_16 as u32)) as u16
+    }
 
-  method tests_Nth_u16() {
-    assert NthUint16(0x1230de80,0) == 0x1230;
-    assert NthUint16(0x1230de80,1) == 0xde80;
-  }
+    method tests_Nth_u16() {
+        assert NthUint16(0x1230de80,0) == 0x1230;
+        assert NthUint16(0x1230de80,1) == 0xde80;
+    }
 }
 
 /**
  * Various helper methods related to unsigned 64bit integers.
  */
 module U64 {
-  import opened Int
+    import opened Int
 
-  // Read nth 32bit word out of this u64, where 0 identifies the most
-  // significant word.
-  function method NthUint32(v:u64, k: nat) : u32
-    // Cannot read more than two words!
-  requires k < 2 {
-    if k == 0
-        then (v / (TWO_32 as u64)) as u32
-      else
-        (v % (TWO_32 as u64)) as u32
-  }
+    // Read nth 32bit word out of this u64, where 0 identifies the most
+    // significant word.
+    function method NthUint32(v:u64, k: nat) : u32
+        // Cannot read more than two words!
+    requires k < 2 {
+        if k == 0
+            then (v / (TWO_32 as u64)) as u32
+        else
+            (v % (TWO_32 as u64)) as u32
+    }
 
-  method testsNthUint32() {
-    assert NthUint32(0x00112233_44556677,0) == 0x00112233;
-    assert NthUint32(0x00112233_44556677,1) == 0x44556677;
-  }
+    method testsNthUint32() {
+        assert NthUint32(0x00112233_44556677,0) == 0x00112233;
+        assert NthUint32(0x00112233_44556677,1) == 0x44556677;
+    }
 }
 
 /**
  * Various helper methods related to unsigned 128bit integers.
  */
 module U128 {
-  import opened Int
+    import opened Int
 
-  // Read nth 64bit word out of this u128, where 0 identifies the most
-  // significant word.
-  function method NthUint64(v:u128, k: nat) : u64
-    // Cannot read more than two words!
-  requires k < 2 {
-    if k == 0
-        then (v / (TWO_64 as u128)) as u64
-      else
-        (v % (TWO_64 as u128)) as u64
-  }
+    // Read nth 64bit word out of this u128, where 0 identifies the most
+    // significant word.
+    function method NthUint64(v:u128, k: nat) : u64
+        // Cannot read more than two words!
+    requires k < 2 {
+        if k == 0
+            then (v / (TWO_64 as u128)) as u64
+        else
+            (v % (TWO_64 as u128)) as u64
+    }
 
-  method testsNthUint64() {
-    assert NthUint64(0x0011223344556677_8899AABBCCDDEEFF,0) == 0x0011223344556677;
-    assert NthUint64(0x0011223344556677_8899AABBCCDDEEFF,1) == 0x8899AABBCCDDEEFF;
-  }
+    method testsNthUint64() {
+        assert NthUint64(0x0011223344556677_8899AABBCCDDEEFF,0) == 0x0011223344556677;
+        assert NthUint64(0x0011223344556677_8899AABBCCDDEEFF,1) == 0x8899AABBCCDDEEFF;
+    }
 }
 
 /**
  * Various helper methods related to unsigned 256bit integers.
  */
 module U256 {
-  import opened Int
-  import U128
-  import U64
-  import U32
-  import U16
+    import opened Int
+    import U128
+    import U64
+    import U32
+    import U16
 
-  // Read nth 128bit word out of this u256, where 0 identifies the most
-  // significant word.
-  function method NthUint128(v:u256, k: nat) : u128
-    // Cannot read more than two words!
-    requires k < 2 {
-      if k == 0
-        then (v / (TWO_128 as u256)) as u128
-      else
-        (v % (TWO_128 as u256)) as u128
-  }
+    function method Shl(lhs: u256, rhs: u256) : u256 {
+        var lbv := lhs as bv256;
+        // NOTE: unclear whether shifting is optimal choice here.
+        var res := if rhs < 256 then (lbv << rhs) else 0;
+        //
+        res as u256
+    }
 
-  // Read nth byte out of this u256, where 0 identifies the most
-  // significant byte.
-  function method NthUint8(v:u256, k: nat) : u8
-    // Cannot read more than 32bytes!
-    requires k < 32 {
-      // This is perhaps a tad ugly.  Happy to take suggestions on
-      // a better approach :)
-      var w128 := NthUint128(v,k / 16);
-      var w64 := U128.NthUint64(w128,(k % 16) / 8);
-      var w32 :=  U64.NthUint32(w64,(k % 8) / 4);
-      var w16 :=  U32.NthUint16(w32,(k % 4) / 2);
-      U16.NthUint8(w16,k%2)
-  }
+    function method Shr(lhs: u256, rhs: u256) : u256 {
+        var lbv := lhs as bv256;
+        // NOTE: unclear whether shifting is optimal choice here.
+        var res := if rhs < 256 then (lbv >> rhs) else 0;
+        //
+        res as u256
+    }
 
-  method testsNthUint128() {
-    assert NthUint128(0x00112233445566778899AABBCCDDEEFF_FFEEDDCCBBAA99887766554433221100,0) == 0x00112233445566778899AABBCCDDEEFF;
-    assert NthUint128(0x00112233445566778899AABBCCDDEEFF_FFEEDDCCBBAA99887766554433221100,1) == 0xFFEEDDCCBBAA99887766554433221100;
-  }
+    // Read nth 128bit word out of this u256, where 0 identifies the most
+    // significant word.
+    function method NthUint128(v:u256, k: nat) : u128
+        // Cannot read more than two words!
+        requires k < 2 {
+        if k == 0
+            then (v / (TWO_128 as u256)) as u128
+        else
+            (v % (TWO_128 as u256)) as u128
+    }
 
-  method testsNthUint8() {
-    assert NthUint8(0x000102030405060708090A0B0C0D0E0F_101112131415161718191A1B1C1D1E1F,00) == 0x00;
-    assert NthUint8(0x000102030405060708090A0B0C0D0E0F_101112131415161718191A1B1C1D1E1F,01) == 0x01;
-    assert NthUint8(0x000102030405060708090A0B0C0D0E0F_101112131415161718191A1B1C1D1E1F,02) == 0x02;
-    assert NthUint8(0x000102030405060708090A0B0C0D0E0F_101112131415161718191A1B1C1D1E1F,03) == 0x03;
-    assert NthUint8(0x000102030405060708090A0B0C0D0E0F_101112131415161718191A1B1C1D1E1F,04) == 0x04;
-    assert NthUint8(0x000102030405060708090A0B0C0D0E0F_101112131415161718191A1B1C1D1E1F,05) == 0x05;
-    assert NthUint8(0x000102030405060708090A0B0C0D0E0F_101112131415161718191A1B1C1D1E1F,06) == 0x06;
-    assert NthUint8(0x000102030405060708090A0B0C0D0E0F_101112131415161718191A1B1C1D1E1F,07) == 0x07;
-    assert NthUint8(0x000102030405060708090A0B0C0D0E0F_101112131415161718191A1B1C1D1E1F,08) == 0x08;
-    assert NthUint8(0x000102030405060708090A0B0C0D0E0F_101112131415161718191A1B1C1D1E1F,09) == 0x09;
-    assert NthUint8(0x000102030405060708090A0B0C0D0E0F_101112131415161718191A1B1C1D1E1F,10) == 0x0A;
-    assert NthUint8(0x000102030405060708090A0B0C0D0E0F_101112131415161718191A1B1C1D1E1F,11) == 0x0B;
-    assert NthUint8(0x000102030405060708090A0B0C0D0E0F_101112131415161718191A1B1C1D1E1F,12) == 0x0C;
-    assert NthUint8(0x000102030405060708090A0B0C0D0E0F_101112131415161718191A1B1C1D1E1F,13) == 0x0D;
-    assert NthUint8(0x000102030405060708090A0B0C0D0E0F_101112131415161718191A1B1C1D1E1F,14) == 0x0E;
-    assert NthUint8(0x000102030405060708090A0B0C0D0E0F_101112131415161718191A1B1C1D1E1F,15) == 0x0F;
-    //
-    assert NthUint8(0x000102030405060708090A0B0C0D0E0F_101112131415161718191A1B1C1D1E1F,16) == 0x10;
-    assert NthUint8(0x000102030405060708090A0B0C0D0E0F_101112131415161718191A1B1C1D1E1F,17) == 0x11;
-    assert NthUint8(0x000102030405060708090A0B0C0D0E0F_101112131415161718191A1B1C1D1E1F,18) == 0x12;
-    assert NthUint8(0x000102030405060708090A0B0C0D0E0F_101112131415161718191A1B1C1D1E1F,19) == 0x13;
-    assert NthUint8(0x000102030405060708090A0B0C0D0E0F_101112131415161718191A1B1C1D1E1F,20) == 0x14;
-    assert NthUint8(0x000102030405060708090A0B0C0D0E0F_101112131415161718191A1B1C1D1E1F,21) == 0x15;
-    assert NthUint8(0x000102030405060708090A0B0C0D0E0F_101112131415161718191A1B1C1D1E1F,22) == 0x16;
-    assert NthUint8(0x000102030405060708090A0B0C0D0E0F_101112131415161718191A1B1C1D1E1F,23) == 0x17;
-    assert NthUint8(0x000102030405060708090A0B0C0D0E0F_101112131415161718191A1B1C1D1E1F,24) == 0x18;
-    assert NthUint8(0x000102030405060708090A0B0C0D0E0F_101112131415161718191A1B1C1D1E1F,25) == 0x19;
-    assert NthUint8(0x000102030405060708090A0B0C0D0E0F_101112131415161718191A1B1C1D1E1F,26) == 0x1A;
-    assert NthUint8(0x000102030405060708090A0B0C0D0E0F_101112131415161718191A1B1C1D1E1F,27) == 0x1B;
-    assert NthUint8(0x000102030405060708090A0B0C0D0E0F_101112131415161718191A1B1C1D1E1F,28) == 0x1C;
-    assert NthUint8(0x000102030405060708090A0B0C0D0E0F_101112131415161718191A1B1C1D1E1F,29) == 0x1D;
-    assert NthUint8(0x000102030405060708090A0B0C0D0E0F_101112131415161718191A1B1C1D1E1F,30) == 0x1E;
-    assert NthUint8(0x000102030405060708090A0B0C0D0E0F_101112131415161718191A1B1C1D1E1F,31) == 0x1F;
+    // Read nth byte out of this u256, where 0 identifies the most
+    // significant byte.
+    function method NthUint8(v:u256, k: nat) : u8
+        // Cannot read more than 32bytes!
+        requires k < 32 {
+        // This is perhaps a tad ugly.  Happy to take suggestions on
+        // a better approach :)
+        var w128 := NthUint128(v,k / 16);
+        var w64 := U128.NthUint64(w128,(k % 16) / 8);
+        var w32 :=  U64.NthUint32(w64,(k % 8) / 4);
+        var w16 :=  U32.NthUint16(w32,(k % 4) / 2);
+        U16.NthUint8(w16,k%2)
+    }
 
-  }
+    method testsNthUint128() {
+        assert NthUint128(0x00112233445566778899AABBCCDDEEFF_FFEEDDCCBBAA99887766554433221100,0) == 0x00112233445566778899AABBCCDDEEFF;
+        assert NthUint128(0x00112233445566778899AABBCCDDEEFF_FFEEDDCCBBAA99887766554433221100,1) == 0xFFEEDDCCBBAA99887766554433221100;
+    }
+
+    method testsNthUint8() {
+        assert NthUint8(0x000102030405060708090A0B0C0D0E0F_101112131415161718191A1B1C1D1E1F,00) == 0x00;
+        assert NthUint8(0x000102030405060708090A0B0C0D0E0F_101112131415161718191A1B1C1D1E1F,01) == 0x01;
+        assert NthUint8(0x000102030405060708090A0B0C0D0E0F_101112131415161718191A1B1C1D1E1F,02) == 0x02;
+        assert NthUint8(0x000102030405060708090A0B0C0D0E0F_101112131415161718191A1B1C1D1E1F,03) == 0x03;
+        assert NthUint8(0x000102030405060708090A0B0C0D0E0F_101112131415161718191A1B1C1D1E1F,04) == 0x04;
+        assert NthUint8(0x000102030405060708090A0B0C0D0E0F_101112131415161718191A1B1C1D1E1F,05) == 0x05;
+        assert NthUint8(0x000102030405060708090A0B0C0D0E0F_101112131415161718191A1B1C1D1E1F,06) == 0x06;
+        assert NthUint8(0x000102030405060708090A0B0C0D0E0F_101112131415161718191A1B1C1D1E1F,07) == 0x07;
+        assert NthUint8(0x000102030405060708090A0B0C0D0E0F_101112131415161718191A1B1C1D1E1F,08) == 0x08;
+        assert NthUint8(0x000102030405060708090A0B0C0D0E0F_101112131415161718191A1B1C1D1E1F,09) == 0x09;
+        assert NthUint8(0x000102030405060708090A0B0C0D0E0F_101112131415161718191A1B1C1D1E1F,10) == 0x0A;
+        assert NthUint8(0x000102030405060708090A0B0C0D0E0F_101112131415161718191A1B1C1D1E1F,11) == 0x0B;
+        assert NthUint8(0x000102030405060708090A0B0C0D0E0F_101112131415161718191A1B1C1D1E1F,12) == 0x0C;
+        assert NthUint8(0x000102030405060708090A0B0C0D0E0F_101112131415161718191A1B1C1D1E1F,13) == 0x0D;
+        assert NthUint8(0x000102030405060708090A0B0C0D0E0F_101112131415161718191A1B1C1D1E1F,14) == 0x0E;
+        assert NthUint8(0x000102030405060708090A0B0C0D0E0F_101112131415161718191A1B1C1D1E1F,15) == 0x0F;
+        //
+        assert NthUint8(0x000102030405060708090A0B0C0D0E0F_101112131415161718191A1B1C1D1E1F,16) == 0x10;
+        assert NthUint8(0x000102030405060708090A0B0C0D0E0F_101112131415161718191A1B1C1D1E1F,17) == 0x11;
+        assert NthUint8(0x000102030405060708090A0B0C0D0E0F_101112131415161718191A1B1C1D1E1F,18) == 0x12;
+        assert NthUint8(0x000102030405060708090A0B0C0D0E0F_101112131415161718191A1B1C1D1E1F,19) == 0x13;
+        assert NthUint8(0x000102030405060708090A0B0C0D0E0F_101112131415161718191A1B1C1D1E1F,20) == 0x14;
+        assert NthUint8(0x000102030405060708090A0B0C0D0E0F_101112131415161718191A1B1C1D1E1F,21) == 0x15;
+        assert NthUint8(0x000102030405060708090A0B0C0D0E0F_101112131415161718191A1B1C1D1E1F,22) == 0x16;
+        assert NthUint8(0x000102030405060708090A0B0C0D0E0F_101112131415161718191A1B1C1D1E1F,23) == 0x17;
+        assert NthUint8(0x000102030405060708090A0B0C0D0E0F_101112131415161718191A1B1C1D1E1F,24) == 0x18;
+        assert NthUint8(0x000102030405060708090A0B0C0D0E0F_101112131415161718191A1B1C1D1E1F,25) == 0x19;
+        assert NthUint8(0x000102030405060708090A0B0C0D0E0F_101112131415161718191A1B1C1D1E1F,26) == 0x1A;
+        assert NthUint8(0x000102030405060708090A0B0C0D0E0F_101112131415161718191A1B1C1D1E1F,27) == 0x1B;
+        assert NthUint8(0x000102030405060708090A0B0C0D0E0F_101112131415161718191A1B1C1D1E1F,28) == 0x1C;
+        assert NthUint8(0x000102030405060708090A0B0C0D0E0F_101112131415161718191A1B1C1D1E1F,29) == 0x1D;
+        assert NthUint8(0x000102030405060708090A0B0C0D0E0F_101112131415161718191A1B1C1D1E1F,30) == 0x1E;
+        assert NthUint8(0x000102030405060708090A0B0C0D0E0F_101112131415161718191A1B1C1D1E1F,31) == 0x1F;
+
+    }
 }
 
 module I256 {
-  import opened Int
+    import U256
+    import Word
+    import opened Int
 
-  // This provides a non-Euclidean division operator and is necessary
-  // because Dafny (unlike just about every other programming
-  // language) supports Euclidean division.  This operator, therefore,
-  // always divides *towards* zero.
-  function method div(lhs: i256, rhs: i256) : i256
-    // Cannot divide by zero!
-    requires rhs != 0
-    // Range restriction to prevent overflow
-    requires (rhs != -1 || lhs != (-TWO_255 as i256)) {
-    Int.Div(lhs as int, rhs as int) as i256
-  }
+    // This provides a non-Euclidean division operator and is necessary
+    // because Dafny (unlike just about every other programming
+    // language) supports Euclidean division.  This operator, therefore,
+    // always divides *towards* zero.
+    function method div(lhs: i256, rhs: i256) : i256
+        // Cannot divide by zero!
+        requires rhs != 0
+        // Range restriction to prevent overflow
+        requires (rhs != -1 || lhs != (-TWO_255 as i256)) {
+        Int.Div(lhs as int, rhs as int) as i256
+    }
 
-  // This provides a non-Euclidean Remainder operator and is necessary
-  // because Dafny (unlike just about every other programming
-  // language) supports Euclidean division.  Observe that this is a
-  // true Remainder operator, and not a modulus operator.  For
-  // emxaple, this means the result can be negative.
-  function method Rem(lhs: i256, rhs: i256) : i256
-    // Cannot divide by zero!
-    requires rhs != 0 {
-    Int.Rem(lhs as int, rhs as int) as i256
-  }
+    // This provides a non-Euclidean Remainder operator and is necessary
+    // because Dafny (unlike just about every other programming
+    // language) supports Euclidean division.  Observe that this is a
+    // true Remainder operator, and not a modulus operator.  For
+    // emxaple, this means the result can be negative.
+    function method Rem(lhs: i256, rhs: i256) : i256
+        // Cannot divide by zero!
+        requires rhs != 0 {
+        Int.Rem(lhs as int, rhs as int) as i256
+    }
+
+    // Shift Arithmetic Right using Bitshifts
+    function method Sar(lhs: i256, rhs: u256) : u256 {
+        if lhs >= 0 then
+            // Easy case, unsigned shr sufficient.
+            U256.Shr(lhs as u256, rhs)
+        else if rhs > 256 then MAX_U256 as u256
+        else
+            // Determine mask
+            var mask := (MAX_U256 as bv256) << (256 - rhs);
+            var lbv := (Word.fromI256(lhs) as bv256 >> rhs);
+            (mask | lbv) as u256
+    }
+
+    // Shift Arithmetic Right.  This implementation follows the Yellow Paper quite
+    // accurately.  However, it performs very poorly when translated into Java.
+    function method Sar2(lhs: i256, rhs: u256) : i256 {
+        if rhs == 0 then lhs
+        else
+            var r := Int.Pow(2,rhs as nat);
+            lemma_pow2(rhs as nat);
+            ((lhs as int) / r) as i256
+    }
 }
 
 module Word {
